tutorial/+rc+/t11_tree_set/code.v
@@ -853,7 +853,7 @@ Section code.
   |}.
 
   (* Definition of function [insert_rec]. *)
-  Definition impl_insert_rec (node insert_rec : loc): function := {|
+  Definition impl_insert_rec (insert_rec node : loc): function := {|
     f_args := [
       ("t", LPtr);
       ("k", it_layout size_t)
@@ -1057,7 +1057,7 @@ Section code.
   |}.
 
   (* Definition of function [remove]. *)
-  Definition impl_remove (free tree_max remove : loc): function := {|
+  Definition impl_remove (free remove tree_max : loc): function := {|
     f_args := [
       ("t", LPtr);
       ("k", it_layout size_t)
@@ -1165,7 +1165,7 @@ Section code.
   |}.
 
   (* Definition of function [main]. *)
-  Definition impl_main (empty init free_tree member insert remove : loc): function := {|
+  Definition impl_main (empty free_tree init insert member remove : loc): function := {|
     f_args := [
     ];
     f_local_vars := [
