examples/+rc+/mpool/proof_mpool_alloc_contiguous_no_fallback.v
@@ -10,11 +10,11 @@ Section proof_mpool_alloc_contiguous_no_fallback.
   Context `{!lockG Σ}.
 
   (* Typing proof for [mpool_alloc_contiguous_no_fallback]. *)
-  Lemma type_mpool_alloc_contiguous_no_fallback (sl_lock sl_unlock round_pointer_up : loc) :
+  Lemma type_mpool_alloc_contiguous_no_fallback (round_pointer_up sl_lock sl_unlock : loc) :
+    round_pointer_up ◁ᵥ round_pointer_up @ function_ptr type_of_round_pointer_up -∗
     sl_lock ◁ᵥ sl_lock @ function_ptr type_of_sl_lock -∗
     sl_unlock ◁ᵥ sl_unlock @ function_ptr type_of_sl_unlock -∗
-    round_pointer_up ◁ᵥ round_pointer_up @ function_ptr type_of_round_pointer_up -∗
-    typed_function (impl_mpool_alloc_contiguous_no_fallback sl_lock sl_unlock round_pointer_up) type_of_mpool_alloc_contiguous_no_fallback.
+    typed_function (impl_mpool_alloc_contiguous_no_fallback round_pointer_up sl_lock sl_unlock) type_of_mpool_alloc_contiguous_no_fallback.
   Proof.
     start_function "mpool_alloc_contiguous_no_fallback" ([[[[[p q] n] entry_size] count] align]) => arg_p arg_count arg_align local_prev local_before_start local_chunk_next local_new_chunk local_start local_ret local_chunk_size local_chunk.
     split_blocks ((
