tutorial/+rc+/t08_tree/proof_remove.v
@@ -9,11 +9,11 @@ Section proof_remove.
   Context `{!typeG Σ} `{!globalG Σ}.
 
   (* Typing proof for [remove]. *)
-  Lemma type_remove (free tree_max remove : loc) :
+  Lemma type_remove (free remove tree_max : loc) :
     free ◁ᵥ free @ function_ptr type_of_free -∗
-    tree_max ◁ᵥ tree_max @ function_ptr type_of_tree_max -∗
     remove ◁ᵥ remove @ function_ptr type_of_remove -∗
-    typed_function (impl_remove free tree_max remove) type_of_remove.
+    tree_max ◁ᵥ tree_max @ function_ptr type_of_tree_max -∗
+    typed_function (impl_remove free remove tree_max) type_of_remove.
   Proof.
     start_function "remove" ([[p t] k]) => arg_t arg_k local_m local_tmp.
     split_blocks ((
